No hope...

theories/Algorithmic/Typing/Definitions.v
@@ -1,74 +1,81 @@
+From Mctt.Algorithmic Require Export IR.
 From Mctt.Algorithmic.Subtyping Require Export Definitions.
 From Mctt.Core Require Import Base.
-Import Domain_Notations.
+Import Syntax_Notations.
+Import IR_Notations.
 
-Reserved Notation "Γ '⊢a' M ⟹ A" (in custom judg at level 80, Γ custom exp, M custom exp, A custom nf).
-Reserved Notation "Γ '⊢a' M ⟸ A" (in custom judg at level 80, Γ custom exp, M custom exp, A custom exp).
+Reserved Notation "Γ '⊢ai' M ⟹ A" (in custom judg at level 80, Γ custom exp, M custom ir, A custom nf).
+Reserved Notation "Γ '⊢ai' M ⟸ A" (in custom judg at level 80, Γ custom exp, M custom ir, A custom exp).
 
 Generalizable All Variables.
 
-Inductive alg_type_check : ctx -> typ -> exp -> Prop :=
+Inductive alg_type_check : ctx -> typ -> ir -> Prop :=
 | atc_ati :
-  `( {{ Γ ⊢a M ⟹ A }} ->
+  `( {{ Γ ⊢ai M ⟹ A }} ->
      {{ Γ ⊢a A ⊆ B }} ->
-     {{ Γ ⊢a M ⟸ B }} )
-where "Γ '⊢a' M ⟸ A" := (alg_type_check Γ A M) (in custom judg) : type_scope
-with alg_type_infer : ctx -> nf -> exp -> Prop :=
+     {{ Γ ⊢ai M ⟸ B }} )
+where "Γ '⊢ai' M ⟸ A" := (alg_type_check Γ A M) (in custom judg) : type_scope
+with alg_type_infer : ctx -> nf -> ir -> Prop :=
 | ati_typ :
-  `( {{ Γ ⊢a Type@i ⟹ Type@(S i) }} )
+  `( {{ Γ ⊢ai Type@i ⟹ Type@(S i) }} )
 | ati_nat :
-  `( {{ Γ ⊢a ℕ ⟹ Type@0 }} )
+  `( {{ Γ ⊢ai ℕ ⟹ Type@0 }} )
 | ati_zero :
-  `( {{ Γ ⊢a zero ⟹ ℕ }} )
+  `( {{ Γ ⊢ai zero ⟹ ℕ }} )
 | ati_succ :
-  `( {{ Γ ⊢a M ⟸ ℕ }} ->
-     {{ Γ ⊢a succ M ⟹ ℕ }} )
+  `( {{ Γ ⊢ai M ⟸ ℕ }} ->
+     {{ Γ ⊢ai succ M ⟹ ℕ }} )
 | ati_natrec :
-  `( {{ Γ, ℕ ⊢a A ⟹ Type@i }} ->
-     {{ Γ ⊢a MZ ⟸ A[Id,,zero] }} ->
-     {{ Γ, ℕ, A ⊢a MS ⟸ A[Wk∘Wk,,succ #1] }} ->
-     {{ Γ ⊢a M ⟸ ℕ }} ->
+  `( {{ Γ, ℕ ⊢ai A ⟹ Type@i }} ->
+     {{ Γ ⊢ai MZ ⟸ A[Id,,zero] }} ->
+     {{ Γ, ℕ, ^(A : typ) ⊢ai MS ⟸ A[Wk∘Wk,,succ #1] }} ->
+     {{ Γ ⊢ai M ⟸ ℕ }} ->
      nbe_ty Γ {{{ A[Id,,M] }}} B ->
-     {{ Γ ⊢a rec M return A | zero -> MZ | succ -> MS end ⟹ B }} )
+     {{ Γ ⊢ai rec M return A | zero -> MZ | succ -> MS end ⟹ B }} )
 | ati_pi :
-  `( {{ Γ ⊢a A ⟹ Type@i }} ->
-     {{ Γ, A ⊢a B ⟹ Type@j }} ->
-     {{ Γ ⊢a Π A B ⟹ Type@(max i j) }} )
+  `( {{ Γ ⊢ai A ⟹ Type@i }} ->
+     {{ Γ, ^(A : typ) ⊢ai B ⟹ Type@j }} ->
+     {{ Γ ⊢ai Π A B ⟹ Type@(max i j) }} )
 | ati_fn :
-  `( {{ Γ ⊢a A ⟹ Type@i }} ->
-     {{ Γ, A ⊢a M ⟹ B }} ->
+  `( {{ Γ ⊢ai A ⟹ Type@i }} ->
+     {{ Γ, ^(A : typ) ⊢ai M ⟹ B }} ->
      nbe_ty Γ A C ->
-     {{ Γ ⊢a λ A M ⟹ Π C B }} )
+     {{ Γ ⊢ai λ A M ⟹ Π C B }} )
 | ati_app :
-  `( {{ Γ ⊢a M ⟹ Π A B }} ->
-     {{ Γ ⊢a N ⟸ A }} ->
+  `( {{ Γ ⊢ai M ⟹ Π A B }} ->
+     {{ Γ ⊢ai N ⟸ A }} ->
      nbe_ty Γ {{{ B[Id,,N] }}} C ->
-     {{ Γ ⊢a M N ⟹ C }} )
+     {{ Γ ⊢ai M N ⟹ C }} )
 | ati_eq :
-  `( {{ Γ ⊢a A ⟹ Type@i }} ->
-     {{ Γ ⊢a M1 ⟸ A }} ->
-     {{ Γ ⊢a M2 ⟸ A }} ->
-     {{ Γ ⊢a Eq A M1 M2 ⟹ Type@i }} )
+  `( {{ Γ ⊢ai A ⟹ Type@i }} ->
+     {{ Γ ⊢ai M1 ⟸ A }} ->
+     {{ Γ ⊢ai M2 ⟸ A }} ->
+     {{ Γ ⊢ai Eq A M1 M2 ⟹ Type@i }} )
 | ati_refl :
-  `( {{ Γ ⊢a A ⟹ Type@i }} ->
-     {{ Γ ⊢a M ⟸ A }} ->
+  `( {{ Γ ⊢ai A ⟹ Type@i }} ->
+     {{ Γ ⊢ai M ⟸ A }} ->
      nbe_ty Γ A C ->
      nbe Γ M A N ->
-     {{ Γ ⊢a refl A M ⟹ Eq C N N }} )
+     {{ Γ ⊢ai refl A M ⟹ Eq C N N }} )
 | ati_eqrec :
-  `( {{ Γ ⊢a A ⟹ Type@i }} ->
-     {{ Γ ⊢a M1 ⟸ A }} ->
-     {{ Γ ⊢a M2 ⟸ A }} ->
-     {{ Γ, A, A[Wk], Eq A[Wk∘Wk] #1 #0 ⊢a B ⟹ Type@j }} ->
-     {{ Γ, A ⊢a BR ⟸ B[Id,,#0,,refl A[Wk] #0] }} ->
-     {{ Γ ⊢a N ⟸ Eq A M1 M2 }} ->
+  `( {{ Γ ⊢ai A ⟹ Type@i }} ->
+     {{ Γ ⊢ai M1 ⟸ A }} ->
+     {{ Γ ⊢ai M2 ⟸ A }} ->
+     {{ Γ, ^(A : typ), A[Wk], Eq A[Wk∘Wk] #1 #0 ⊢ai B ⟹ Type@j }} ->
+     {{ Γ, ^(A : typ) ⊢ai BR ⟸ B[Id,,#0,,refl A[Wk] #0] }} ->
+     {{ Γ ⊢ai N ⟸ Eq A M1 M2 }} ->
      nbe_ty Γ {{{ B[Id,,M1,,M2,,N] }}} C ->
-     {{ Γ ⊢a eqrec N as Eq A M1 M2 return B | refl -> BR end ⟹ C }} )
+     {{ Γ ⊢ai eqrec N as Eq A M1 M2 return B | refl -> BR end ⟹ C }} )
 | ati_vlookup :
   `( {{ #x : A ∈ Γ }} ->
      nbe_ty Γ A B ->
-     {{ Γ ⊢a #x ⟹ B }} )
-where "Γ '⊢a' M ⟹ A" := (alg_type_infer Γ A M) (in custom judg) : type_scope.
+     {{ Γ ⊢ai #x ⟹ B }} )
+| ati_ann :
+  `( {{ Γ ⊢ai A ⟹ Type@i }} ->
+     {{ Γ ⊢ai M ⟸ A }} ->
+     nbe_ty Γ A B ->
+     {{ Γ ⊢ai M : A ⟹ B }} )
+where "Γ '⊢ai' M ⟹ A" := (alg_type_infer Γ A M) (in custom judg) : type_scope.
 
 #[export]
 Hint Constructors alg_type_check alg_type_infer : mctt.
