theories/Algorithmic/Typing/Lemmas.v
@@ -7,10 +7,11 @@ From Mctt.Core.Semantic Require Import Consequences.
 From Mctt.Core.Soundness Require Import EqualityCases.
 From Mctt.Frontend Require Import Elaborator.
 Import Domain_Notations.
+Import IR_Notations.
 
 Lemma functional_alg_type_infer : forall {Γ A A' M},
-    {{ Γ ⊢a M ⟹ A }} ->
-    {{ Γ ⊢a M ⟹ A' }} ->
+    {{ Γ ⊢ai M ⟹ A }} ->
+    {{ Γ ⊢ai M ⟹ A' }} ->
     A = A'.
 Proof.
   intros * HM1 HM2. gen A'.
@@ -20,7 +21,7 @@ Proof.
     f_equiv;
     try reflexivity;
     intuition.
-  - assert (n{{{ Type@i }}} = n{{{ Type@i0 }}}) as [= <-] by intuition.
+  -  assert (n{{{ Type@i }}} = n{{{ Type@i0 }}}) as [= <-] by intuition.
     assert (n{{{ Type@j }}} = n{{{ Type@j0 }}}) as [= <-] by intuition.
     reflexivity.
   - assert (n{{{ Π A B }}} = n{{{ Π A0 B0 }}}) as [= <- <-] by intuition.
@@ -39,14 +40,14 @@ Hint Resolve functional_alg_type_infer : mctt.
 Ltac functional_alg_type_infer_rewrite_clear1 :=
   let tactic_error o1 o2 := fail 3 "functional_alg_type_infer equality between" o1 "and" o2 "cannot be solved by mauto" in
   match goal with
-  | H1 : {{ ^?Γ ⊢a ^?M ⟹ ^?A1 }}, H2 : {{ ^?Γ ⊢a ^?M ⟹ ^?A2 }} |- _ =>
+  | H1 : {{ ^?Γ ⊢ai ^?M ⟹ ^?A1 }}, H2 : {{ ^?Γ ⊢ai ^?M ⟹ ^?A2 }} |- _ =>
       clean replace A2 with A1 by first [solve [mauto 2 using functional_alg_type_infer] | tactic_error A2 A1]; clear H2
   end.
 Ltac functional_alg_type_infer_rewrite_clear := repeat functional_alg_type_infer_rewrite_clear1.
 
 Lemma alg_type_sound :
-  (forall {Γ A M}, {{ Γ ⊢a M ⟸ A }} -> {{ ⊢ Γ }} -> forall i, {{ Γ ⊢ A : Type@i }} -> {{ Γ ⊢ M : A }}) /\
-    (forall {Γ A M}, {{ Γ ⊢a M ⟹ A }} -> {{ ⊢ Γ }} -> {{ Γ ⊢ M : A }}).
+  (forall {Γ A M}, {{ Γ ⊢ai M ⟸ A }} -> {{ ⊢ Γ }} -> forall i, {{ Γ ⊢ A : Type@i }} -> {{ Γ ⊢ M : A }}) /\
+    (forall {Γ A M}, {{ Γ ⊢ai M ⟹ A }} -> {{ ⊢ Γ }} -> {{ Γ ⊢ M : A }}).
 Proof.
   apply alg_type_mut_ind; intros; try mautosolve 4.
   - assert {{ Γ ⊢ M : A }} by mauto 3.
@@ -58,25 +59,25 @@ Proof.
   - assert {{ Γ ⊢ ℕ : Type@0 }} by mauto 2.
     assert {{ ⊢ Γ, ℕ }} by mauto 2.
     assert {{ Γ, ℕ ⊢ A : Type@i }} by mauto 2.
-    assert {{ ⊢ Γ, ℕ, A }} by mauto 3.
+    assert {{ ⊢ Γ, ℕ, ^(A : typ) }} by mauto 3.
     assert {{ Γ ⊢ M : ℕ }} by mauto 2.
     assert {{ Γ ⊢ A[Id,,zero] : Type@i }} by mauto 3.
-    assert {{ Γ, ℕ, A ⊢ A[Wk∘Wk,,succ #1] : Type@i }} by mauto 3.
+    assert {{ Γ, ℕ, ^(A : typ) ⊢ A[Wk∘Wk,,succ #1] : Type@i }} by mauto 3.
     assert {{ Γ ⊢ A[Id,,M] ≈ B : Type@i }} as <- by mauto 4 using soundness_ty'.
     mauto 4.
   - assert {{ Γ ⊢ A : Type@i }} by mauto 2.
-    assert {{ ⊢ Γ, A }} by mauto 3.
+    assert {{ ⊢ Γ, ^(A : typ) }} by mauto 3.
     mauto 3.
   - assert {{ Γ ⊢ A : Type@i }} by mauto 2.
-    assert {{ ⊢ Γ, A }} by mauto 3.
+    assert {{ ⊢ Γ, ^(A : typ) }} by mauto 3.
     assert {{ Γ ⊢ A ≈ C : Type@i }} by mauto 2 using soundness_ty'.
-    assert {{ Γ, A ⊢ M : B }} by mauto 2.
-    assert (exists j, {{ Γ, A ⊢ B : Type@j }}) as [j] by (gen_presups; eauto 2).
+    assert {{ Γ, ^(A : typ) ⊢ M : B }} by mauto 2.
+    assert (exists j, {{ Γ, ^(A : typ) ⊢ B : Type@j }}) as [j] by (gen_presups; eauto 2).
     assert {{ Γ ⊢ Π A B ≈ Π C B : Type@(max i j) }} as <- by mauto 3.
     mauto 3.
   - assert {{ Γ ⊢ M : Π A B }} by mauto 2.
     assert (exists i, {{ Γ ⊢ Π A B : Type@i }}) as [i] by (gen_presups; eauto 2).
-    assert ({{ Γ ⊢ A : Type@i }} /\ {{ Γ, ^(A : exp) ⊢ B : Type@i }}) as [] by mauto 3.
+    assert ({{ Γ ⊢ A : Type@i }} /\ {{ Γ, ^(A : typ) ⊢ B : Type@i }}) as [] by mauto 3.
     assert {{ Γ ⊢ N : A }} by mauto 2.
     assert {{ Γ ⊢ B[Id,,N] ≈ C : Type@i }} as <- by mauto 4 using soundness_ty'.
     mauto 3.
@@ -94,12 +95,12 @@ Proof.
   - assert {{ Γ ⊢ A : Type@i }} by mauto 2.
     assert {{ Γ ⊢ M1 : A }} by mauto 2.
     assert {{ Γ ⊢ M2 : A }} by mauto 2.
-    assert {{ ⊢ Γ, A }} by mauto 2.
-    assert {{ Γ, A ⊢s Wk : Γ }} by mauto 2.
-    assert {{ Γ, A ⊢ A[Wk] : Type@i }} by mauto 2.
-    assert {{ Γ, A, A[Wk] ⊢ Eq A[Wk∘Wk] #1 #0 : Type@i }} by mauto 2.
-    assert {{ ⊢ Γ, A, A[Wk], Eq A[Wk∘Wk] #1 #0 }} by mauto 3.
-    assert {{ Γ, A, A[Wk], Eq A[Wk∘Wk] #1 #0 ⊢ B : Type@j }} by mauto 2.
+    assert {{ ⊢ Γ, ^(A : typ) }} by mauto 2.
+    assert {{ Γ, ^(A : typ) ⊢s Wk : Γ }} by mauto 2.
+    assert {{ Γ, ^(A : typ) ⊢ A[Wk] : Type@i }} by mauto 2.
+    assert {{ Γ, ^(A : typ), A[Wk] ⊢ Eq A[Wk∘Wk] #1 #0 : Type@i }} by mauto 2.
+    assert {{ ⊢ Γ, ^(A : typ), A[Wk], Eq A[Wk∘Wk] #1 #0 }} by mauto 3.
+    assert {{ Γ, ^(A : typ), A[Wk], Eq A[Wk∘Wk] #1 #0 ⊢ B : Type@j }} by mauto 2.
     unshelve epose proof (@glu_rel_eq_eqrec_synprop_gen _ {{{ Id }}} _ _ A _ _); shelve_unifiable; [| eassumption |]; mauto 3;
       destruct_conjs.
     assert {{ Γ ⊢ M1 : A[Id] }} by mauto 2.
@@ -108,9 +109,9 @@ Proof.
     | H : forall _ _, _ -> _ -> _ |- _ =>
          unshelve epose proof (H M1 M2 _ _); shelve_unifiable; [eassumption | eassumption |]; destruct_conjs
     end.
-    assert {{ Γ, A ⊢ BR : B[Id,,#0,,refl A[Wk] #0] }} by mauto 3.
+    assert {{ Γ, ^(A : typ) ⊢ BR : B[Id,,#0,,refl A[Wk] #0] }} by mauto 3.
     assert {{ Γ ⊢ N : Eq A M1 M2 }} by mauto 3.
-    assert {{ Γ ⊢s Id,,M1,,M2,,N : Γ, A, A[Wk], Eq A[Wk∘Wk] #1 #0 }} by mauto 2.
+    assert {{ Γ ⊢s Id,,M1,,M2,,N : Γ, ^(A : typ), A[Wk], Eq A[Wk∘Wk] #1 #0 }} by mauto 2.
     assert {{ Γ ⊢ B[Id,,M1,,M2,,N] : Type@j }} by mauto 2.
     assert {{ Γ ⊢ B[Id,,M1,,M2,,N] ≈ C : Type@j }} as <- by mauto 2 using soundness_ty'.
     mauto 3.
@@ -118,10 +119,13 @@ Proof.
     assert (exists i, {{ Γ ⊢ A : Type@i }}) as [i] by mauto 2.
     assert {{ Γ ⊢ A ≈ B : Type@i }} as <- by mauto 2 using soundness_ty'.
     mauto 3.
+  - assert {{ Γ ⊢ A : Type@i }} by mauto 2.
+    assert {{ Γ ⊢ A ≈ B : Type@i }} by mauto 2 using soundness_ty'.
+    mauto 3.
 Qed.
 
 Lemma alg_type_check_sound : forall {Γ i A M},
-    {{ Γ ⊢a M ⟸ A }} ->
+    {{ Γ ⊢ai M ⟸ A }} ->
     {{ ⊢ Γ }} ->
     {{ Γ ⊢ A : Type@i }} ->
     {{ Γ ⊢ M : A }}.
@@ -130,14 +134,14 @@ Proof.
 Qed.
 
 Lemma alg_type_infer_sound : forall {Γ A M},
-    {{ Γ ⊢a M ⟹ A }} -> {{ ⊢ Γ }} -> {{ Γ ⊢ M : A }}.
+    {{ Γ ⊢ai M ⟹ A }} -> {{ ⊢ Γ }} -> {{ Γ ⊢ M : A }}.
 Proof.
   pose proof alg_type_sound; intuition.
 Qed.
 
 Lemma alg_type_infer_normal : forall {Γ A A' M},
     {{ ⊢ Γ }} ->
-    {{ Γ ⊢a M ⟹ A }} ->
+    {{ Γ ⊢ai M ⟹ A }} ->
     nbe_ty Γ A A' ->
     A = A'.
 Proof with (f_equiv; mautosolve 4).
@@ -154,22 +158,22 @@ Proof with (f_equiv; mautosolve 4).
     assert {{ Γ, ℕ ⊢ A : ^n{{{ Type@i }}} }} by mauto 3 using alg_type_infer_sound...
   - assert {{ Γ ⊢ A : ^n{{{ Type@i }}} }} by mauto 3 using alg_type_infer_sound.
     assert {{ Γ ⊢ A ≈ C : Type@i }} by mauto 3 using soundness_ty'.
-    assert {{ Γ, A ⊢ M : B }} by mauto 3 using alg_type_infer_sound.
-    assert (exists j, {{ Γ, A ⊢ B : Type@j }}) as [j] by (gen_presups; eauto 2).
-    assert {{ ⊢ Γ, A ≈ Γ, ^(C : exp) }} by mauto 3.
+    assert {{ Γ, ^(A : typ) ⊢ M : B }} by mauto 3 using alg_type_infer_sound.
+    assert (exists j, {{ Γ, ^(A : typ) ⊢ B : Type@j }}) as [j] by (gen_presups; eauto 2).
+    assert {{ ⊢ Γ, ^(A : typ) ≈ Γ, ^(C : typ) }} by mauto 3.
     dir_inversion_clear_by_head nbe_ty.
     simplify_evals.
     dir_inversion_by_head read_typ; subst.
     functional_initial_env_rewrite_clear.
-    assert (initial_env {{{ Γ, ^(C : exp) }}} d{{{ ρ ↦ ⇑! a (length Γ) }}}) by mauto 3.
+    assert (initial_env {{{ Γ, ^(C : typ) }}} d{{{ ρ ↦ ⇑! a (length Γ) }}}) by mauto 3.
     assert (nbe_ty Γ A C) by mauto 3.
     assert (nbe_ty Γ C A0) by mauto 3.
     replace A0 with C by mauto 2.
-    assert (nbe_ty {{{ Γ, ^(C : exp) }}} B B') by mauto 3.
-    assert (nbe_ty {{{ Γ, A }}} B B') by mauto 4 using ctxeq_nbe_ty_eq'...
+    assert (nbe_ty {{{ Γ, ^(C : typ) }}} B B') by mauto 3.
+    assert (nbe_ty {{{ Γ, ^(A : typ) }}} B B') by mauto 4 using ctxeq_nbe_ty_eq'...
   - assert {{ Γ ⊢ M : ^n{{{ Π A B }}} }} by mauto 3 using alg_type_infer_sound.
     assert (exists i, {{ Γ ⊢ Π A B : Type@i }}) as [i] by (gen_presups; eauto 2).
-    assert ({{ Γ ⊢ A : Type@i }} /\ {{ Γ, ^(A : exp) ⊢ B : Type@i }}) as [] by mauto 3.
+    assert ({{ Γ ⊢ A : Type@i }} /\ {{ Γ, ^(A : typ) ⊢ B : Type@i }}) as [] by mauto 3.
     assert {{ Γ ⊢ N : A }} by mauto 3 using alg_type_check_sound.
     assert {{ Γ ⊢ B[Id,,N] : Type@i }} by mauto 3...
   - assert {{ Γ ⊢ A : ^n{{{ Type@i }}} }} by mauto 3 using alg_type_infer_sound.
@@ -192,15 +196,16 @@ Proof with (f_equiv; mautosolve 4).
     assert {{ Γ ⊢ M1 : A }} by mauto 3 using alg_type_check_sound.
     assert {{ Γ ⊢ M2 : A }} by mauto 3 using alg_type_check_sound.
     assert {{ Γ ⊢ N : Eq A M1 M2 }} by mauto 3 using alg_type_check_sound.
-    assert {{ Γ, A ⊢s Wk : Γ }} by mauto 3.
-    assert {{ Γ, A ⊢ A[Wk] : Type@i }} by mauto 3.
-    assert {{ ⊢ Γ, A, A[Wk] }} by mauto 3.
-    assert {{ Γ, A, A[Wk] ⊢ Eq A[Wk∘Wk] #1 #0 : Type@i }} by mauto 3.
-    assert {{ Γ, A, A[Wk], Eq A[Wk∘Wk] #1 #0 ⊢ B : ^n{{{ Type@j }}} }} by mauto 3 using alg_type_infer_sound.
-    assert {{ Γ ⊢s Id,,M1,,M2,,N : Γ, A, A[Wk], Eq A[Wk∘Wk] #1 #0 }} by mauto 2.
+    assert {{ Γ, ^(A : typ) ⊢s Wk : Γ }} by mauto 3.
+    assert {{ Γ, ^(A : typ) ⊢ A[Wk] : Type@i }} by mauto 3.
+    assert {{ ⊢ Γ, ^(A : typ), A[Wk] }} by mauto 3.
+    assert {{ Γ, ^(A : typ), A[Wk] ⊢ Eq A[Wk∘Wk] #1 #0 : Type@i }} by mauto 3.
+    assert {{ Γ, ^(A : typ), A[Wk], Eq A[Wk∘Wk] #1 #0 ⊢ B : ^n{{{ Type@j }}} }} by mauto 3 using alg_type_infer_sound.
+    assert {{ Γ ⊢s Id,,M1,,M2,,N : Γ, ^(A : typ), A[Wk], Eq A[Wk∘Wk] #1 #0 }} by mauto 2.
     assert {{ Γ ⊢ B[Id,,M1,,M2,,N] : Type@j }} by mauto 2.
     mauto 3.
   - assert (exists i, {{ Γ ⊢ A : Type@i }}) as [i] by mauto 2...
+  - assert {{ Γ ⊢ A : ^n{{{ Type@i }}} }} by mauto 3 using alg_type_infer_sound...
 Qed.
 
 #[export]
@@ -208,8 +213,8 @@ Hint Resolve alg_type_infer_normal : mctt.
 
 Lemma alg_type_check_typ_implies_alg_type_infer_typ : forall {Γ A i},
     {{ ⊢ Γ }} ->
-    {{ Γ ⊢a A ⟸ Type@i }} ->
-    exists j, {{ Γ ⊢a A ⟹ Type@j }} /\ j <= i.
+    {{ Γ ⊢ai A ⟸ Type@i }} ->
+    exists j, {{ Γ ⊢ai A ⟹ Type@j }} /\ j <= i.
 Proof.
   intros * ? Hcheck.
   inversion Hcheck as [? A' ? ? Hinfer Hsub]; subst.
@@ -228,8 +233,8 @@ Hint Resolve alg_type_check_typ_implies_alg_type_infer_typ : mctt.
 Lemma alg_type_check_pi_implies_alg_type_infer_pi : forall {Γ M A B i},
     {{ ⊢ Γ }} ->
     {{ Γ ⊢ Π A B : Type@i }} ->
-    {{ Γ ⊢a M ⟸ Π A B }} ->
-    exists A' B', {{ Γ ⊢a M ⟹ Π A' B' }} /\ {{ Γ ⊢ A' ≈ A : Type@i }} /\ {{ Γ, A ⊢a B' ⊆ B }}.
+    {{ Γ ⊢ai M ⟸ Π A B }} ->
+    exists A' B', {{ Γ ⊢ai M ⟹ Π A' B' }} /\ {{ Γ ⊢ A' ≈ A : Type@i }} /\ {{ Γ, A ⊢a B' ⊆ B }}.
 Proof.
   intros * ? ? Hcheck.
   assert ({{ Γ ⊢ A : Type@i }} /\ {{ Γ, A ⊢ B : Type@i }}) as [] by mauto 3.
@@ -265,9 +270,9 @@ Qed.
 Hint Resolve alg_type_check_pi_implies_alg_type_infer_pi : mctt.
 
 Lemma alg_type_check_subtyp : forall {Γ A A' M},
-    {{ Γ ⊢a M ⟸ A }} ->
+    {{ Γ ⊢ai M ⟸ A }} ->
     {{ Γ ⊢ A ⊆ A' }} ->
-    {{ Γ ⊢a M ⟸ A' }}.
+    {{ Γ ⊢ai M ⟸ A' }}.
 Proof.
   intros * [] **.
   assert {{ Γ0 ⊢a B ⊆ A' }} by mauto 3 using alg_subtyping_complete.
@@ -278,9 +283,9 @@ Qed.
 Hint Resolve alg_type_check_subtyp : mctt.
 
 Corollary alg_type_check_conv : forall {Γ i A A' M},
-    {{ Γ ⊢a M ⟸ A }} ->
+    {{ Γ ⊢ai M ⟸ A }} ->
     {{ Γ ⊢ A ≈ A' : Type@i }} ->
-    {{ Γ ⊢a M ⟸ A' }}.
+    {{ Γ ⊢ai M ⟸ A' }}.
 Proof.
   mauto 3.
 Qed.
@@ -289,28 +294,38 @@ Qed.
 Hint Resolve alg_type_check_conv : mctt.
 
 Lemma alg_type_check_complete : forall {Γ A M},
-    user_exp M ->
     {{ Γ ⊢ M : A }} ->
-    {{ Γ ⊢a M ⟸ A }}.
+    exists M', {{ Γ ⊢ai M' ⟸ A }} /\ M = M'.
 Proof.
-  intros * Hue.
-  induction 1; gen_presups; inversion Hue; subst; clear Hue; mauto 4 using alg_subtyping_complete, alg_type_check_subtyp.
-  - econstructor; mauto 3.
-    unshelve solve [mauto using alg_subtyping_complete]; constructor.
+  intros * H.
+  dependent induction H; gen_presups; [> try (eexists; split; [mauto 4 using alg_subtyping_complete, alg_type_check_subtyp | reflexivity]) ..].
+  - exists i{{{ zero }}}; split; [| reflexivity].
+    econstructor; mauto 3.
+    mauto 4 using alg_subtyping_complete, alg_type_check_subtyp.
+  - destruct_all; subst.
+    eexists i{{{ succ ^_ }}}; split; [| reflexivity].
+    econstructor; mauto 3.
+    mauto 4 using alg_subtyping_complete, alg_type_check_subtyp.
+  - destruct_all; subst.
+    eexists i{{{ rec ^_ return ^_ | zero -> ^_ | succ -> ^_ end }}}; split; [| reflexivity].
+    econstructor; mauto 3.
+    + econstructor; mauto 3.
+      * 
+    + apply alg_subtyping_complete. unshelve solve [mauto using alg_subtyping_complete]; constructor.
   - econstructor; mauto 3.
     mauto using alg_subtyping_complete.
-  - assert (exists j, {{ Γ, ℕ ⊢a A ⟹ Type@j }} /\ j <= i) as [j []] by mauto 3.
+  - assert (exists j, {{ Γ, ℕ ⊢ai A ⟹ Type@j }} /\ j <= i) as [j []] by mauto 3.
     assert {{ Γ ⊢ A[Id,,M] : Type@i }} by mauto 3.
     assert {{ Γ ⊢ A[Id,,M] ≈ A[Id,,M] : Type@i }} as [? [? _]]%completeness_ty by mauto 3.
     econstructor; mauto using alg_subtyping_complete, soundness_ty'.
-  - assert (exists j, {{ Γ ⊢a A ⟹ Type@j }} /\ j <= i) as [j []] by mauto 3.
+  - assert (exists j, {{ Γ ⊢ai A ⟹ Type@j }} /\ j <= i) as [j []] by mauto 3.
     assert {{ ⊢ Γ, A }} by mauto 3.
-    assert (exists j, {{ Γ, A ⊢a B ⟹ Type@j }} /\ j <= i) as [j' []] by mauto 3.
+    assert (exists j, {{ Γ, A ⊢ai B ⟹ Type@j }} /\ j <= i) as [j' []] by mauto 3.
     assert (max j j' <= i) by lia.
     econstructor; mauto 3 using alg_subtyping_complete.
-  - assert (exists j, {{ Γ ⊢a A ⟹ Type@j }} /\ j <= i) as [j []] by mauto 3.
-    assert {{ Γ, A ⊢a M ⟸ B }} by mauto 3.
-    assert (exists B', {{ Γ, A ⊢a M ⟹ B' }} /\ {{ Γ, A ⊢a B' ⊆ B }}) as [B' []] by (inversion_clear_by_head alg_type_check; firstorder).
+  - assert (exists j, {{ Γ ⊢ai A ⟹ Type@j }} /\ j <= i) as [j []] by mauto 3.
+    assert {{ Γ, A ⊢ai M ⟸ B }} by mauto 3.
+    assert (exists B', {{ Γ, A ⊢ai M ⟹ B' }} /\ {{ Γ, A ⊢a B' ⊆ B }}) as [B' []] by (inversion_clear_by_head alg_type_check; firstorder).
     assert (exists W, nbe_ty Γ A W /\ {{ Γ ⊢ A ≈ W : Type@i }}) as [W []] by mauto 3 using soundness_ty.
     assert {{ ⊢ Γ, A }} by mauto 3.
     assert {{ Γ, A ⊢ M : B' }} by mauto 3 using alg_type_infer_sound.
@@ -319,9 +334,9 @@ Proof.
     eapply alg_subtyping_complete.
     eapply wf_subtyp_pi'; mauto 2.
     mauto 4 using alg_subtyping_sound, lift_exp_max_left, lift_exp_max_right.
-  - assert {{ Γ ⊢a M ⟸ Π A B }} by mauto 2.
-    assert {{ Γ ⊢a N ⟸ A }} by mauto 2.
-    assert (exists A' B', {{ Γ ⊢a M ⟹ Π A' B' }} /\ {{ Γ ⊢ A' ≈ A : Type@i }} /\ {{ Γ, A ⊢a B' ⊆ B }}) as [A' [B' [? []]]] by mauto 3.
+  - assert {{ Γ ⊢ai M ⟸ Π A B }} by mauto 2.
+    assert {{ Γ ⊢ai N ⟸ A }} by mauto 2.
+    assert (exists A' B', {{ Γ ⊢ai M ⟹ Π A' B' }} /\ {{ Γ ⊢ A' ≈ A : Type@i }} /\ {{ Γ, A ⊢a B' ⊆ B }}) as [A' [B' [? []]]] by mauto 3.
     assert {{ Γ ⊢ M : ^n{{{ Π A' B' }}} }} by mauto 3 using alg_type_infer_sound.
     assert (exists j, {{ Γ ⊢ Π A' B' : Type@j }}) as [j] by (gen_presups; eauto 2).
     assert ({{ Γ ⊢ A' : Type@j }} /\ {{ Γ, ^(A' : exp) ⊢ B' : Type@j }}) as [] by mauto 3.
@@ -335,17 +350,17 @@ Proof.
     econstructor; mauto 4 using alg_subtyping_complete.
   - assert (exists W, nbe_ty Γ A W /\ {{ Γ ⊢ A ≈ W : Type@i }}) as [W []] by (eapply soundness_ty; mauto 3).
     econstructor; mauto 4 using alg_subtyping_complete.
-  - assert (exists j, {{ Γ ⊢a A ⟹ Type@j }} /\ j <= i) as [j []] by mauto 3.
+  - assert (exists j, {{ Γ ⊢ai A ⟹ Type@j }} /\ j <= i) as [j []] by mauto 3.
     econstructor; [econstructor |]; mauto 3 using alg_subtyping_complete.
-  - assert (exists j, {{ Γ ⊢a A ⟹ Type@j }} /\ j <= i) as [j []] by mauto 3.
-    assert {{ Γ ⊢a M ⟸ A }} by eauto 2.
+  - assert (exists j, {{ Γ ⊢ai A ⟹ Type@j }} /\ j <= i) as [j []] by mauto 3.
+    assert {{ Γ ⊢ai M ⟸ A }} by eauto 2.
     assert (exists C, nbe_ty Γ A C /\ {{ Γ ⊢ A ≈ C : Type@i }}) as [C []] by mauto 3 using soundness_ty.
     assert (exists W, nbe Γ M A W /\ {{ Γ ⊢ M ≈ W : A }}) as [W []] by mauto 3 using soundness.
     econstructor; mauto 3.
     assert {{ Γ ⊢ ^n{{{ Eq C W W }}} ≈ Eq A M M : Type@i }} by mauto 3.
     mauto 3 using alg_subtyping_complete.
-  - assert (exists k, {{ Γ ⊢a A ⟹ Type@k }} /\ k <= i) as [k []] by mauto 3.
-    assert (exists l, {{ Γ, A, A[Wk], Eq A[Wk∘Wk] #1 #0 ⊢a B ⟹ Type@l }} /\ l <= j) as [l []] by mauto 3.
+  - assert (exists k, {{ Γ ⊢ai A ⟹ Type@k }} /\ k <= i) as [k []] by mauto 3.
+    assert (exists l, {{ Γ, A, A[Wk], Eq A[Wk∘Wk] #1 #0 ⊢ai B ⟹ Type@l }} /\ l <= j) as [l []] by mauto 3.
     assert {{ Γ, A ⊢s Wk : Γ }} by mauto 3.
     assert {{ Γ, A ⊢ A[Wk] : Type@i }} by mauto 3.
     assert {{ ⊢ Γ, A, A[Wk] }} by mauto 3.
@@ -363,10 +378,10 @@ Hint Resolve alg_type_check_complete : mctt.
 Corollary alg_type_infer_complete : forall {Γ A M},
     user_exp M ->
     {{ Γ ⊢ M : A }} ->
-    exists B, {{ Γ ⊢a M ⟹ B }} /\ {{ Γ ⊢a B ⊆ A }}.
+    exists B, {{ Γ ⊢ai M ⟹ B }} /\ {{ Γ ⊢a B ⊆ A }}.
 Proof.
   intros.
-  assert {{ Γ ⊢a M ⟸ A }} as Hcheck by mauto 4 using alg_type_check_complete.
+  assert {{ Γ ⊢ai M ⟸ A }} as Hcheck by mauto 4 using alg_type_check_complete.
   inversion_clear Hcheck.
   firstorder.
 Qed.
@@ -377,7 +392,7 @@ Hint Resolve alg_type_infer_complete : mctt.
 Corollary alg_type_infer_typ_complete : forall {Γ i A},
     user_exp A ->
     {{ Γ ⊢ A : Type@i }} ->
-    exists j, {{ Γ ⊢a A ⟹ Type@j }} /\ j <= i.
+    exists j, {{ Γ ⊢ai A ⟹ Type@j }} /\ j <= i.
 Proof.
   mauto 4 using alg_type_check_complete.
 Qed.
@@ -388,7 +403,7 @@ Hint Resolve alg_type_infer_typ_complete : mctt.
 Corollary alg_type_infer_pi_complete : forall {Γ i A},
     user_exp A ->
     {{ Γ ⊢ A : Type@i }} ->
-    exists j, {{ Γ ⊢a A ⟹ Type@j }} /\ j <= i.
+    exists j, {{ Γ ⊢ai A ⟹ Type@j }} /\ j <= i.
 Proof.
   mauto 4 using alg_type_check_complete.
 Qed.
